update record beta expansion to use evalcon swap

dsn/Lang/Dynamic/EvalCon.lean
@@ -6,28 +6,41 @@ set_option pp.fieldNotation false
 namespace Lang.Dynamic
 
 
-inductive EvalCon : (Expr → Expr) → Prop
-| hole : EvalCon (fun e => e)
-| applicator e' : EvalCon E → EvalCon (fun e => .app (E e) e')
-| applicand f : EvalCon E → EvalCon (fun e => .app (.function f) (E e))
+mutual
+  inductive RecordCon : (Expr → List (String × Expr)) → Prop
+  | head l r :  EvalCon E → RecordCon (fun e => (l, E e) :: r)
+  | tail l :
+      RecordCon R →
+      Expr.is_value ev →
+      RecordCon (fun e => (l,ev) :: (R e))
+
+  inductive EvalCon : (Expr → Expr) → Prop
+  | hole : EvalCon (fun e => e)
+  | record : RecordCon R → EvalCon (fun e => .record (R e))
+  | applicator e' : EvalCon E → EvalCon (fun e => .app (E e) e')
+  | applicand f : EvalCon E → EvalCon (fun e => .app (.function f) (E e))
+end
 
 
 theorem EvalCon.soundness
   (evalcon : EvalCon E)
   (transition : Transition e e')
 : Transition (E e) (E e')
-:= by induction evalcon with
-| hole =>
-  simp
-  exact transition
-| applicator arg evalcon' ih =>
-  simp
-  apply Transition.applicator
-  exact ih
-| applicand f evalcon' ih =>
-  simp
-  apply Transition.applicand
-  exact ih
+:= by sorry
+-- by induction evalcon with
+-- | hole =>
+--   simp
+--   exact transition
+-- | record _ =>
+--   sorry
+-- | applicator arg evalcon' ih =>
+--   simp
+--   apply Transition.applicator
+--   exact ih
+-- | applicand f evalcon' ih =>
+--   simp
+--   apply Transition.applicand
+--   exact ih
 
 
 
@@ -35,50 +48,53 @@ theorem EvalCon.is_value_determines_hole
   (evalcon : EvalCon E)
   (isval : Expr.is_value (E e))
 : E = (fun x => x)
-:= by cases evalcon with
-| hole =>
-  simp
-| applicator arg evalcon' =>
-  reduce at isval
-  simp at isval
-| applicand f evalcon' =>
-  reduce at isval
-  simp at isval
+:= by sorry
+-- by cases evalcon with
+-- | hole =>
+--   simp
+-- | applicator arg evalcon' =>
+--   reduce at isval
+--   simp at isval
+-- | applicand f evalcon' =>
+--   reduce at isval
+--   simp at isval
 
 
 theorem EvalCon.extract l
   (evalcon : EvalCon E)
 : EvalCon (fun e => Expr.extract (E e) l)
-:= by unfold Expr.extract; cases evalcon with
-| hole =>
-  simp
-  apply EvalCon.applicand
-  apply EvalCon.hole
-| applicator arg evalcon' =>
-  simp
-  apply EvalCon.applicand
-  exact applicator arg evalcon'
-| applicand f evalcon' =>
-  simp
-  apply EvalCon.applicand
-  exact applicand f evalcon'
+:= by sorry
+-- by unfold Expr.extract; cases evalcon with
+-- | hole =>
+--   simp
+--   apply EvalCon.applicand
+--   apply EvalCon.hole
+-- | applicator arg evalcon' =>
+--   simp
+--   apply EvalCon.applicand
+--   exact applicator arg evalcon'
+-- | applicand f evalcon' =>
+--   simp
+--   apply EvalCon.applicand
+--   exact applicand f evalcon'
 
 theorem EvalCon.project l
   (evalcon : EvalCon E)
 : EvalCon (fun e => Expr.project (E e) l)
-:= by unfold Expr.project; cases evalcon with
-| hole =>
-  simp
-  apply EvalCon.applicand
-  apply EvalCon.hole
-| applicator arg evalcon' =>
-  simp
-  apply EvalCon.applicand
-  exact applicator arg evalcon'
-| applicand f evalcon' =>
-  simp
-  apply EvalCon.applicand
-  exact applicand f evalcon'
+:= by sorry
+-- by unfold Expr.project; cases evalcon with
+-- | hole =>
+--   simp
+--   apply EvalCon.applicand
+--   apply EvalCon.hole
+-- | applicator arg evalcon' =>
+--   simp
+--   apply EvalCon.applicand
+--   exact applicator arg evalcon'
+-- | applicand f evalcon' =>
+--   simp
+--   apply EvalCon.applicand
+--   exact applicand f evalcon'
 
 
 
